Wasm_Big_Step.thy
@@ -98,7 +98,7 @@ inductive reduce_to :: "[(s \<times> v list \<times> e list), (nat list \<times>
 | local_trap:"\<lbrakk>(s,lls,es) \<Down>{([],Some n,j)} (s',lls',RTrap)\<rbrakk> \<Longrightarrow> (s,vs,[Local n j lls es]) \<Down>{\<Gamma>} (s',vs,RTrap)"
   \<comment> \<open>\<open>break congruence\<close>\<close>
 | label_break_suc:"\<lbrakk>(s,vs,es) \<Down>{(n#ls,r,i)} (s',vs',RBreak (Suc bn) bvs)\<rbrakk> \<Longrightarrow> (s,vs,[Label n les es]) \<Down>{(ls,r,i)} (s',vs',RBreak bn bvs)"
-| label_break_nil:"\<lbrakk>(s,vs,es) \<Down>{(n#ls,r,i)} (s',vs',RBreak 0 bvs)\<rbrakk> \<Longrightarrow> (s,vs,[Label n les es]) \<Down>{(ls,r,i)} (s',vs',RValue bvs)"
+| label_break_nil:"\<lbrakk>(s,vs,es) \<Down>{(n#ls,r,i)} (s'',vs'',RBreak 0 bvs); (s'',vs'',($$* bvs) @ es') \<Down>{\<Gamma>} (s',vs',res)\<rbrakk> \<Longrightarrow> (s,vs,[Label n les es]) \<Down>{(ls,r,i)} (s',vs',res)"
   \<comment> \<open>\<open>return congruence\<close>\<close>
 | label_return:"\<lbrakk>(s,vs,es) \<Down>{(n#ls,r,i)} (s',vs',RReturn rvs)\<rbrakk> \<Longrightarrow> (s,vs,[Label n les es]) \<Down>{(ls,r,i)} (s',vs',RReturn rvs)"
 | local_return:"\<lbrakk>(s,lls,es) \<Down>{([],Some n,j)} (s',lls',RReturn rvs)\<rbrakk> \<Longrightarrow> (s,vs,[Local n j lls es]) \<Down>{\<Gamma>} (s',vs,RValue rvs)"
@@ -195,7 +195,7 @@ inductive reduce_to_n :: "[(s \<times> v list \<times> e list), nat, (nat list \
 | local_trap:"\<lbrakk>(s,lls,es) \<Down>k{([],Some n,j)} (s',lls',RTrap)\<rbrakk> \<Longrightarrow> (s,vs,[Local n j lls es]) \<Down>k{\<Gamma>} (s',vs,RTrap)"
   \<comment> \<open>\<open>break congruence\<close>\<close>
 | label_break_suc:"\<lbrakk>(s,vs,es) \<Down>k{(n#ls,r,i)} (s',vs',RBreak (Suc bn) bvs)\<rbrakk> \<Longrightarrow> (s,vs,[Label n les es]) \<Down>k{(ls,r,i)} (s',vs',RBreak bn bvs)"
-| label_break_nil:"\<lbrakk>(s,vs,es) \<Down>k{(n#ls,r,i)} (s',vs',RBreak 0 bvs)\<rbrakk> \<Longrightarrow> (s,vs,[Label n les es]) \<Down>k{(ls,r,i)} (s',vs',RValue bvs)"
+| label_break_nil:"\<lbrakk>(s,vs,es) \<Down>k{(n#ls,r,i)} (s'',vs'',RBreak 0 bvs); (s'',vs'',($$* bvs) @ es') \<Down>k{\<Gamma>} (s',vs',res)\<rbrakk> \<Longrightarrow> (s,vs,[Label n les es]) \<Down>k{(ls,r,i)} (s',vs',res)"
   \<comment> \<open>\<open>return congruence\<close>\<close>
 | label_return:"\<lbrakk>(s,vs,es) \<Down>k{(n#ls,r,i)} (s',vs',RReturn rvs)\<rbrakk> \<Longrightarrow> (s,vs,[Label n les es]) \<Down>k{(ls,r,i)} (s',vs',RReturn rvs)"
 | local_return:"\<lbrakk>(s,lls,es) \<Down>k{([],Some n,j)} (s',lls',RReturn rvs)\<rbrakk> \<Longrightarrow> (s,vs,[Local n j lls es]) \<Down>k{\<Gamma>} (s',vs,RValue rvs)"
@@ -220,6 +220,12 @@ proof (induction rule: reduce_to.induct)
   thus ?case
     using reduce_to_n_mono reduce_to_n.seq_value
     by (meson le_cases)
+next
+  case (label_break_nil s vs es n ls r i s'' vs'' bvs es' \<Gamma> s' vs' res les)
+  thus ?case
+    using reduce_to_n_mono reduce_to_n.label_break_nil
+    by (meson le_cases)
+next
 qed (fastforce intro: reduce_to_n.intros)+
 
 lemma reduce_to_n_imp_reduce_to:
